changed TraceM to use function graphs; almost finished the proofs that TraceM is a monad

theories/TraceMonad.v
@@ -9,7 +9,75 @@ Import ListNotations.
  *** The Trace Monad = Final Algebra of Sets of Traces
  ***)
 
-Definition TraceM St `{OType St} A `{OType A} :
-  St -> DownSet (list St * option A).
+(* A trace computation starts from any given input state, and generates a trace
+of intermediate states followed by an optional final state (if it terminates) *)
+Definition TraceM St `{OType St} A `{OType A} :=
+  FunGraph St (list St * option (A * St)).
 
-FIXME HERE: finish this!
+Instance OTypeF_TraceM St `{OType St} : OTypeF (TraceM St) := fun _ _ => _.
+
+Instance MonadOps_TraceM St `{OType St} : MonadOps (TraceM St) :=
+  {| returnM :=
+       fun _ _ x =>
+         (* For each input st, return x as the output and st as the final state,
+         with no intermediate states *)
+         lambdaDownSet (fun st => downClose ([], Some (x, st)));
+     bindM :=
+       fun _ _ _ _ m f =>
+         (* For each input state st... *)
+         lambdaDownSet
+           (fun st =>
+              bindDownSet
+                (* Pass st into m *)
+                (applyDownSet m st)
+                (fun trace_out1 =>
+                   (* Get (trace1, out) = (m st), and test if out is a Some *)
+                   optElim
+                     (fun a_st1 =>
+                        (* If (m st) = (trace1, Some (a, st2)), then get
+                           (trace2, out) = (f a st), and return the result
+                           (trace1 ++ trace2, out) *)
+                        mapDownSet
+                          (fun trace_out2 =>
+                             (fst trace_out1 ++ fst trace_out2, snd trace_out2))
+                          (applyDownSet (f (fst a_st1)) (snd a_st1)))
+                     (* Otherwise, m did not terminate, so we don't call f at
+                     all, and just return (trace1, None) *)
+                     (downClose (fst trace_out1, None))
+                     (* (snd trace_out1) is the option output of (m st) *)
+                     (snd trace_out1)))
+  |}.
+
+Instance Monad_TraceM St `{OType St} : Monad (TraceM St).
+Proof.
+  constructor.
+  { intros. intros a1 a2 Ra. simpl. apply Proper_lambdaDownSet. intro st.
+    rewrite Ra. reflexivity. }
+  { intros. intros m1 m2 Rm f1 f2 Rf. apply Proper_lambdaDownSet. intro st.
+    rewrite Rm. apply Proper_bindDownSet; try reflexivity. intro trace_out1.
+    apply (Proper_optElim_eq _ _); try reflexivity.
+    intro a_st1. apply Proper_bindDownSet; try reflexivity.
+    apply Proper_applyDownSet; [ apply Rf | reflexivity ]. }
+  { intros. simpl.
+    rewrite <- (downSetEta (f a)).
+    apply Proper_lambdaDownSet_equiv. apply funOExt; intro st.
+    rewrite downSetBeta; [ | intros st1 st2 Rst; rewrite Rst; reflexivity ].
+    rewrite DownSet_return_bind.
+    - simpl. unfold mapDownSet.
+      etransitivity; [ | apply DownSet_bind_return ].
+      apply Proper_bindDownSet_equiv; try reflexivity.
+      apply funOExt. intros [ tr ret ]. reflexivity.
+    - intros tr_out1 tr_out2 Rtr_out.
+      eapply Proper_optElim; try (rewrite Rtr_out; reflexivity).
+      intros a_st1 a_st1' Ra_st1.
+      apply Proper_bindDownSet; [ rewrite Ra_st1; reflexivity | ].
+      intro f_tr_out. rewrite Rtr_out. reflexivity. }
+  { intros. simpl. rewrite <- (downSetEta m).
+    apply Proper_lambdaDownSet_equiv. apply funOExt; intro st.
+    etransitivity; [ | apply DownSet_bind_return ].
+    f_equiv. apply funOExt. intros [ tr [[ a st'] | ]]; [ | reflexivity ].
+    simpl. unfold mapDownSet. rewrite downSetBeta.
+    - rewrite DownSet_return_bind; [ simpl; rewrite app_nil_r; reflexivity | ].
+      intros tr_ret1 tr_ret2 Rtr_ret. rewrite Rtr_ret. reflexivity.
+    - intros st1 st2 Rst. rewrite Rst. reflexivity. }
+  { intros.
